lib/translator.ml
@@ -517,20 +517,24 @@ module Translator = struct
         t_fmls_input
         metadata
         = 
-      let original_specs_ensures = 
+      let add_ensures = 
         List.filter 
-          (fun x -> match x with 
-            | AST.TopDecl.Ensures _ -> true 
-            | _  -> false ) original_specs in
-      let original_specs_pre = 
+          (fun x -> 
+            match x with 
+            | AST.TopDecl.Ensures x -> TCommon.is_expr_marked x | _ -> false) 
+        original_specs in
+      let add_ensures = 
+        List.map 
+          (fun x ->
+            match x with 
+            | AST.TopDecl.Ensures x -> TCommon.unmark_expr x | _ -> assert false)
+        add_ensures in    
+      let original_specs = 
         List.filter 
-          (fun x -> match x with 
-            | AST.TopDecl.Ensures _ -> false 
-            | _  -> true ) original_specs in
-      let ensures_exprs = List.map 
-        (fun x -> match x with | AST.TopDecl.Ensures e -> e | _ -> assert false)
-        original_specs_ensures in
-      let ensure_expr = TCommon.expr_lst_to_and ensures_exprs in
+        (fun x -> 
+          match x with 
+          | AST.TopDecl.Ensures x -> not (TCommon.is_expr_marked x) | _ -> true) 
+        original_specs in
       (
         let valids = 
           Refinement.generate_checker_4_fmls 
@@ -542,7 +546,7 @@ module Translator = struct
           fun x -> AST.TopDecl.Requires x
         ) valids
       ) @
-      (List.map t_function_spec original_specs_pre) @ (
+      (List.map t_function_spec original_specs) @ (
         let t_args = get_args_from_fmls t_fmls_input in
         let modes = (
           match metadata with 
@@ -674,10 +678,21 @@ module Translator = struct
             body = TCommon.expr_lst_to_and [
               TCommon.expr_lst_to_and rtn_valids;
               get_self_call_from_func_id_and_args id args_for_l_call;
-              ensure_expr
             ]
           } in
-          [AST.TopDecl.Ensures binding]
+          let add_ensures = List.map 
+            (
+              fun x -> 
+                AST.Prog.Let {
+                  ghost = false;
+                  pats = assignee;
+                  defs = NonEmptyList.coerce [self_call];
+                  body = x
+                }
+            ) add_ensures in
+          let add_ensures = List.map 
+              (fun x -> AST.TopDecl.Ensures x) add_ensures in
+          add_ensures @  [AST.TopDecl.Ensures binding]
         )
       )
       in
